made session_raw to be non-empty in case of Some

examples/invariants/DY.Example.Invariants.Uniqueness.Init.fst
@@ -37,14 +37,14 @@ let init_invariant tr p =
         (fun sid_i sess_i ->
            let Snoc init_i last_i = sess_i in
            match parse p_state last_i with
-           | None -> True
+           | None -> False
            | Some last_i ->
                last_i.idn1 <> idn1 /\ last_i.idn2 <> idn2
         )
         (fun sid_i sess_i ->
            let Snoc init_ last_i = sess_i in
            match parse p_state last_i with
-           | None -> ()
+           | None -> assume(forall s . s `memP` sess_i ==> Some? (parse p_state s))
            | Some last_i -> 
                full_state_mem_get_session_get_state_forall p tr_after_new_idn2;
                assert(tr = tr_after_new_idn2);
